establish n-ary product

theories/typing/product.v
@@ -1,7 +1,8 @@
+Require Import FunctionalExtensionality Equality.
 From iris.proofmode Require Import tactics.
 From iris.algebra Require Import list numbers.
-From lrust.util Require Import basic update.
-From lrust.typing Require Import lft_contexts.
+From lrust.util Require Import basic update types.
+From lrust.typing Require Import lft_contexts mod_ty.
 From lrust.typing Require Export type.
 
 Set Default Proof Using "Type".
@@ -24,155 +25,146 @@ Section product.
     iIntros. iIntros. iApply step_fupdN_intro; [done|]. iIntros "!>!>!>!>!>".
     iExists [], 1%Qp=>/=. iSplit; [iPureIntro; by apply proph_dep_unit|]. by iFrame.
   Qed.
-  Global Instance unit_copy : Copy unit.
+
+  Global Instance unit_copy: Copy unit.
   Proof.
     split; [apply _|]. move=> */=. iIntros "_ _ Na $". iExists 1%Qp, []. iModIntro.
     iDestruct (na_own_acc with "Na") as "[$ ToNa]"; [solve_ndisj|].
     rewrite heap_mapsto_vec_nil. do 2 (iSplit; [done|]). iIntros "?_!>". by iApply "ToNa".
   Qed.
-  Global Instance unit_send : Send unit. Proof. done. Qed.
-  Global Instance unit_sync : Sync unit. Proof. done. Qed.
+  Global Instance unit_send: Send unit. Proof. done. Qed.
+  Global Instance unit_sync: Sync unit. Proof. done. Qed.
 
-  Lemma split_prod_mt {A B} (vπd1: _ A) (vπd2: _ B) tid ty1 ty2 q l :
-    (l ↦∗{q}: λ vl, ∃ vl1 vl2,
-       ⌜vl = vl1 ++ vl2⌝ ∗ ty1.(ty_own) vπd1 tid vl1 ∗ ty2.(ty_own) vπd2 tid vl2)%I
-       ⊣⊢ l ↦∗{q}: ty1.(ty_own) vπd1 tid ∗
-          (l +ₗ ty1.(ty_size)) ↦∗{q}: ty2.(ty_own) vπd2 tid.
+  Lemma split_prod_mt {A B} (vπd: _ A) (vπd': _ B) tid ty ty' q l :
+    (l ↦∗{q}: λ vl, ∃wl wl', ⌜vl = wl ++ wl'⌝ ∗
+      ty.(ty_own) vπd tid wl ∗ ty'.(ty_own) vπd' tid wl')%I ⊣⊢
+    l ↦∗{q}: ty.(ty_own) vπd tid ∗
+      (l +ₗ ty.(ty_size)) ↦∗{q}: ty'.(ty_own) vπd' tid.
   Proof.
-    iSplit; iIntros "H".
-    - iDestruct "H" as (vl) "[H↦ H]". iDestruct "H" as (vl1 vl2 ?) "[H1 H2]".
-      subst. rewrite heap_mapsto_vec_app. iDestruct "H↦" as "[H↦1 H↦2]".
-      iDestruct (ty_size_eq with "H1") as %->.
-      iSplitL "H1 H↦1"; iExists _; iFrame.
-    - iDestruct "H" as "[H1 H2]".
-      iDestruct "H1" as (vl1) "[H↦1 H1]". iDestruct "H2" as (vl2) "[H↦2 H2]".
-      iExists (vl1 ++ vl2). rewrite heap_mapsto_vec_app.
-      iDestruct (ty_size_eq with "H1") as %->. auto with iFrame.
+    iSplit.
+    - iDestruct 1 as (?) "[Mt Own]". iDestruct "Own" as (??->) "[Own Own']".
+      rewrite heap_mapsto_vec_app. iDestruct "Mt" as "[Mt Mt']".
+      iDestruct (ty_size_eq with "Own") as %->.
+      iSplitL "Mt Own"; iExists _; iFrame.
+    - iDestruct 1 as "[Own Own']". iDestruct "Own" as (wl) "[Mt Own]".
+      iDestruct "Own'" as (wl') "[Mt' Own']". iExists (wl ++ wl').
+      rewrite heap_mapsto_vec_app. iDestruct (ty_size_eq with "Own") as %->.
+      iFrame "Mt Mt'". iExists wl, wl'. by iFrame.
   Qed.
 
-  Program Definition product2 {A B} (ty1 : type A) (ty2 : type B) : type (A * B) :=
-    {| ty_size := ty1.(ty_size) + ty2.(ty_size);
-       ty_lfts := ty1.(ty_lfts) ++ ty2.(ty_lfts);  ty_E := ty1.(ty_E) ++ ty2.(ty_E);
-       ty_own vπd tid vl := (∃ vl1 vl2, ⌜vl = vl1 ++ vl2⌝ ∗
-        ty1.(ty_own) (fst ∘ vπd.1, vπd.2) tid vl1 ∗ ty2.(ty_own) (snd ∘ vπd.1, vπd.2) tid vl2)%I;
-       ty_shr d κ tid l := (ty1.(ty_shr) (fst ∘ d.1, d.2) κ tid l ∗
-          ty2.(ty_shr) (snd ∘ d.1, d.2) κ tid (l +ₗ ty1.(ty_size)))%I |}.
+  Program Definition product2 {A B} (ty: type A) (ty': type B) : type (A * B) :=
+    {| ty_size := ty.(ty_size) + ty'.(ty_size);
+       ty_lfts := ty.(ty_lfts) ++ ty'.(ty_lfts);  ty_E := ty.(ty_E) ++ ty'.(ty_E);
+       ty_own vπd tid vl := (∃ wl wl', ⌜vl = wl ++ wl'⌝ ∗
+        ty.(ty_own) (fst ∘ vπd.1, vπd.2) tid wl ∗ ty'.(ty_own) (snd ∘ vπd.1, vπd.2) tid wl')%I;
+       ty_shr vπd κ tid l := (ty.(ty_shr) (fst ∘ vπd.1, vπd.2) κ tid l ∗
+          ty'.(ty_shr) (snd ∘ vπd.1, vπd.2) κ tid (l +ₗ ty.(ty_size)))%I |}.
   Next Obligation.
-    move=> *. iDestruct 1 as (vl1 vl2 ->) "[H1 H2]".
-    rewrite app_length !ty_size_eq.
-    iDestruct "H1" as %->. iDestruct "H2" as %->. done.
+    move=> */=. iDestruct 1 as (??->) "H". rewrite app_length !ty_size_eq.
+    by iDestruct "H" as "[->->]".
   Qed.
   Next Obligation.
-    move=> *. iDestruct 1 as (vl1 vl2 ->) "[H1 H2]".
-    iExists vl1, vl2. iSplit; [done|]. by iSplitL "H1"; iApply ty_own_depth_mono.
+    move=> *. iDestruct 1 as (wl wl' ->) "[Own Own']". iExists wl, wl'.
+    iSplit; [done|]. by iSplitL "Own"; iApply ty_own_depth_mono.
   Qed.
-
   Next Obligation.
     move=> *. iIntros "[??]". iSplit; by iApply ty_shr_depth_mono.
   Qed.
-
   Next Obligation.
-    move=> *. iIntros "Hout [??]". iSplit; by iApply (ty_shr_lft_mono with "Hout").
+    move=> *. iIntros "In [??]". iSplit; by iApply (ty_shr_lft_mono with "In").
   Qed.
-
   Next Obligation.
-    intros A B ty1 ty2 E vπ vπd κ l tid q ?; iIntros "#LFT /= #? H [Htok1 Htok2]".
-    rewrite split_prod_mt.
-
-    iMod (bor_sep with "LFT H") as "[H1 H2]"; first solve_ndisj.
-    iMod (ty1.(ty_share A) with "LFT [] H1 Htok1") as "H1"; first solve_ndisj.
+    move=> */=. iIntros "#LFT #? Own [Tok Tok']". rewrite split_prod_mt.
+    iMod (bor_sep with "LFT Own") as "[Own Own']"; first done.
+    iMod (ty_share with "LFT [] Own Tok") as "Own"; first done.
     { iApply lft_incl_trans; [done|]. rewrite lft_intersect_list_app.
       iApply lft_intersect_incl_l. }
-    iMod (ty2.(ty_share B) with "LFT [] H2 Htok2") as "H2"; first solve_ndisj.
+    iMod (ty_share with "LFT [] Own' Tok'") as "Own'"; first solve_ndisj.
     { iApply lft_incl_trans; [done|]. rewrite lft_intersect_list_app.
       iApply lft_intersect_incl_r. }
-
-    iDestruct (step_fupdN_combine with "H1 H2") as "H1".
-    iModIntro.
-    iApply (step_fupdN_wand with "H1").
-    iIntros "[> [? ?] > [? ?]]". by iFrame.
-    Qed.
-
+    iDestruct (step_fupdN_combine with "Own Own'") as "Own".
+    iApply (step_fupdN_wand with "Own"). by iIntros "!> [>[$$] >[$$]]".
+  Qed.
   Next Obligation.
-    iIntros (A B ty1 ty2 N vπ d tid vl κ q ?) "#LFT #H⊑".
-    iDestruct 1 as (vl1 vl2) "(? & Hownty1 & Hownty2)".
-    iIntros "[Htok1 Htok2]".
-    iDestruct (ty_own_proph with "LFT [] Hownty1 Htok1") as "> H1"; first done.
+    move=> *. iIntros "#LFT #?". iDestruct 1 as (wl wl' ->) "[Own Own']".
+    iIntros "[Tok Tok']".
+    iDestruct (ty_own_proph with "LFT [] Own Tok") as ">Close"; first done.
     { iApply lft_incl_trans; [done|]. rewrite lft_intersect_list_app.
       iApply lft_intersect_incl_l. }
-    iDestruct (ty_own_proph with "LFT [] Hownty2 Htok2") as "> H2"; first done.
+    iDestruct (ty_own_proph with "LFT [] Own' Tok'") as ">Close'"; first done.
     { iApply lft_incl_trans; [done|]. rewrite lft_intersect_list_app.
       iApply lft_intersect_incl_r. }
-
-    iDestruct (step_fupdN_combine with "H1 H2") as "H1".
-    iApply (step_fupdN_wand with "H1").
-    iModIntro.
-    iIntros "[H1 H2]".
-    iMod "H1" as (ξs1 q1') "(% & q1dep & ty1own)".
-    iMod "H2" as (ξs2 q2') "(% & q2dep & ty2own)".
-    destruct (Qp_lower_bound q1' q2') as (x & r1 & r2 & Hq1 & Hq2); setoid_subst.
-    iExists (ξs1 ++ ξs2), x.
-    iModIntro.
-    iSplit.
-    - iPureIntro.
-      by apply proph_dep_pair.
-    - iDestruct "q1dep" as "[xξ1 r1ξ1]".
-      iDestruct "q2dep" as "[xξ2 r2ξ2]".
-      iSplitL "xξ1 xξ2"; iFrame.
-      iIntros "[xξ1 xξ2]".
-      iMod ("ty1own" with "[$]") as "[? ?]"; first iFrame.
-      iMod ("ty2own" with "[$]") as "[? ?]"; first iFrame.
-      iExists vl1, vl2; by iFrame.
+    iDestruct (step_fupdN_combine with "Close Close'") as "Close".
+    iApply (step_fupdN_wand with "Close"). iIntros "!> [Close Close']".
+    iMod "Close" as (ξs q ?) "[PTok Close]". iMod "Close'" as (ξs' q' ?) "[PTok' Close']".
+    iDestruct (proph_tok_combine with "PTok PTok'") as (q0) "[PTok PrePTok]".
+    iExists (ξs ++ ξs'), q0. iModIntro. iSplit. { iPureIntro. by apply proph_dep_pair. }
+    iFrame "PTok". iIntros "PTok". iDestruct ("PrePTok" with "PTok") as "[PTok PTok']".
+    iMod ("Close" with "PTok") as "[?$]". iMod ("Close'" with "PTok'") as "[?$]".
+    iModIntro. iExists wl, wl'. iSplit; [done|]. iFrame.
   Qed.
-
   Next Obligation.
-    iIntros (A B ty1 ty2 E vπ d κ tid l κ' q ?) "/= #LFT #Hsub #? [Hty1 Hty2] [Htok1 Htok2]".
-    iMod (ty1.(ty_shr_proph A) with "LFT Hsub [] Hty1 Htok1") as "Hty1"; first done.
+    move=> *. iIntros "#LFT #In #?". iDestruct 1 as "[Shr Shr']". iIntros "[Tok Tok']".
+    iDestruct (ty_shr_proph with "LFT In [] Shr Tok") as "> Close"; first done.
     { iApply lft_incl_trans; [done|]. rewrite lft_intersect_list_app.
       iApply lft_intersect_incl_l. }
-    iMod (ty2.(ty_shr_proph B) with "LFT Hsub [] Hty2 Htok2") as "Hty2"; first done.
+    iDestruct (ty_shr_proph with "LFT In [] Shr' Tok'") as "> Close'"; first done.
     { iApply lft_incl_trans; [done|]. rewrite lft_intersect_list_app.
       iApply lft_intersect_incl_r. }
-    iModIntro; iNext.
-    iDestruct (step_fupdN_combine with "Hty1 Hty2") as ">>H1".
-    iApply (step_fupdN_wand with "H1").
-    iModIntro.
-    iIntros "[Hty1 Hty2]".
-    iMod "Hty1" as (ξs1 q1') "(% & q1dep & ty1own)".
-    iMod "Hty2" as (ξs2 q2') "(% & q2dep & ty2own)".
-    destruct (Qp_lower_bound q1' q2') as (x & r1 & r2 & -> & ->).
-    iDestruct "q1dep" as "[xξ1 r1ξ1]".
-    iDestruct "q2dep" as "[xξ2 r2ξ2]".
-    iExists (ξs1 ++ ξs2), x.
-    iModIntro.
-    iSplit.
-    - iPureIntro.
-      by apply proph_dep_pair.
-    - iSplitL "xξ1 xξ2"; iFrame.
-      iIntros "[? ?]".
-      iMod ("ty1own" with "[$]") as "[? ?]".
-      iMod ("ty2own" with "[$]") as "[? ?]".
-      by iFrame.
+    iIntros "!>!>". iMod (step_fupdN_combine with "Close Close'") as ">Close".
+    iApply (step_fupdN_wand with "Close"). iIntros "!> [Close Close']".
+    iMod "Close" as (ξs q ?) "[PTok Close]". iMod "Close'" as (ξs' q' ?) "[PTok' Close']".
+    iDestruct (proph_tok_combine with "PTok PTok'") as (q0) "[PTok PrePTok]".
+    iExists (ξs ++ ξs'), q0. iModIntro. iSplit. { iPureIntro. by apply proph_dep_pair. }
+    iFrame "PTok". iIntros "PTok". iDestruct ("PrePTok" with "PTok") as "[PTok PTok']".
+    iMod ("Close" with "PTok") as "[$$]". by iMod ("Close'" with "PTok'") as "[$$]".
   Qed.
 
-  Global Instance product2_lft_morphism {A B C} (T1 : type A → type B) (T2 : type A → type C):
-    TypeLftMorphism T1 → TypeLftMorphism T2 →
-    TypeLftMorphism (λ ty, product2 (T1 ty) (T2 ty)).
+  Global Instance product2_ne {A B} : NonExpansive2 (@product2 A B).
+  Proof. solve_ne_type. Qed.
+
+  Definition nil_unit: type :1 := mod_ty (λ _, -[]) unit.
+
+  Definition cons_product2 {A B} (ty: type A) (ty': type B)
+    : type (A :* B) := mod_ty pair_to_cons_pair (product2 ty ty').
+
+  Global Instance cons_product2_ne {A B} : NonExpansive2 (@cons_product2 A B).
+  Proof. move=> ???????. rewrite /cons_product2. by do 2 f_equiv. Qed.
+
+  Fixpoint product {As} (tyl: typel As) : type (xprod As) :=
+    match tyl with +[] => nil_unit | ty +:: tyl' => cons_product2 ty (product tyl') end.
+
+  Global Instance product_ne {As} : NonExpansive (@product As).
+  Proof. move=> ???. elim; [done|]=> */=. by f_equiv. Qed.
+
+End product.
+
+Notation "ty * ty'" := (product2 ty%T ty'%T) : lrust_type_scope.
+Notation ":1" := nil_unit : lrust_type_scope.
+Notation "ty :* ty'" := (cons_product2 ty%T ty'%T) : lrust_type_scope.
+Notation Π := product.
+
+Section typing.
+  Context `{!typeG Σ}.
+
+  Global Instance product2_lft_morphism {A B C} (T: _ A → _ B) (T' : _ → _ C):
+    TypeLftMorphism T → TypeLftMorphism T' →
+    TypeLftMorphism (λ ty, product2 (T ty) (T' ty)).
   Proof.
-    destruct 1 as [α βs E Hα HE|α E Hα HE], 1 as [α' βs' E' Hα' HE'|α' E' Hα' HE'].
-    - apply (type_lft_morphism_add _ (α ⊓ α') (βs ++ βs') (E ++ E'))=>ty.
+    case=> [α βs E Hα HE|α E Hα HE]; case=> [α' βs' E' Hα' HE'|α' E' Hα' HE'].
+    - apply (type_lft_morphism_add _ (α ⊓ α') (βs ++ βs') (E ++ E'))=> ty.
       + rewrite lft_intersect_list_app. iApply lft_equiv_trans.
         { iApply lft_intersect_equiv_proper; [iApply Hα|iApply Hα']. }
         rewrite -!assoc (comm (⊓) (ty_lft ty) (α' ⊓ _)) -!assoc.
         repeat iApply lft_intersect_equiv_proper; try iApply lft_equiv_refl.
         iApply lft_intersect_equiv_idemp.
       + rewrite /= !elctx_interp_app HE HE' big_sepL_app -!assoc.
-        iSplit; iIntros "#H"; repeat iDestruct "H" as "[? H]"; iFrame "#".
+        iSplit; iIntros "#H"; repeat iDestruct "H" as "[?H]"; iFrame "#".
     - apply (type_lft_morphism_add _ (α ⊓ α') βs (E ++ E'))=>ty.
       + rewrite lft_intersect_list_app -assoc (comm (⊓) α' (ty_lft ty)) assoc.
         iApply lft_intersect_equiv_proper; [iApply Hα|iApply Hα'].
       + rewrite /= !elctx_interp_app HE HE' -!assoc.
-        iSplit; iIntros "#H"; repeat iDestruct "H" as "[? H]"; iFrame "#".
+        iSplit; iIntros "#H"; repeat iDestruct "H" as "[?H]"; iFrame "#".
     - apply (type_lft_morphism_add _ (α ⊓ α') βs' (E ++ E'))=>ty.
       + rewrite lft_intersect_list_app -assoc.
         iApply lft_intersect_equiv_proper; [iApply Hα|iApply Hα'].
@@ -183,165 +175,144 @@ Section product.
       + by rewrite /= !elctx_interp_app HE HE'.
   Qed.
 
-  Global Instance product2_type_ne {A B C} (T1: _ A → _ B) (T2: _ A → _ C) :
-    TypeNonExpansive T1 → TypeNonExpansive T2 →
-    TypeNonExpansive (λ ty, product2 (T1 ty) (T2 ty)).
-  Proof.
-    intros HT1 HT2. split.
-    - apply _.
-    - move=>ty1 ty2 /= ?.
-      rewrite !(type_non_expansive_ty_size (T:=T1) ty1 ty2) //.
-      rewrite !(type_non_expansive_ty_size (T:=T2) ty1 ty2) //.
-    - move=> n ty1 ty2 Hsz Hl HE Ho Hs vπd tid vl /=.
-      by do 6 f_equiv; apply type_non_expansive_ty_own.
-    - move=> n ty1 ty2 Hsz Hl HE Ho Hs κ tid l l' /=.
-      rewrite !(type_non_expansive_ty_size (T:=T1) ty1 ty2) //.
-      by f_equiv; apply type_non_expansive_ty_shr.
+  Global Instance product2_type_ne {A B C} (T: _ A → _ B) (T': _ → _ C) :
+    TypeNonExpansive T → TypeNonExpansive T' → TypeNonExpansive (λ ty, T ty * T' ty)%T.
+  Proof. move=> ??. split=>/=; first apply _.
+    - move=> *. f_equiv; by apply type_non_expansive_ty_size.
+    - move=> *. do 6 f_equiv; by apply type_non_expansive_ty_own.
+    - move=> ? ty ty' *. rewrite (type_non_expansive_ty_size (T:=T) ty ty'); [|done].
+      f_equiv; by apply type_non_expansive_ty_shr.
   Qed.
-
   (* TODO : find a way to avoid this duplication. *)
-  Global Instance product2_type_contractive {A B C} (T1: _ A → _ B) (T2: _ A → _ C) :
-    TypeContractive T1 → TypeContractive T2 →
-    TypeContractive (λ ty, product2 (T1 ty) (T2 ty)).
-  Proof.
-    intros HT1 HT2. split.
-    - apply _.
-    - move=>ty1 ty2 /=.
-      rewrite !(type_contractive_ty_size (T:=T1) ty1 ty2).
-      by rewrite !(type_contractive_ty_size (T:=T2) ty1 ty2).
-    - move=> n ty1 ty2 Hsz Hl HE Ho Hs vπd tid vl /=.
-      by do 6 f_equiv; apply type_contractive_ty_own.
-    - move=> n ty1 ty2 Hsz Hl HE Ho Hs κ tid l l' /=.
-      rewrite !(type_contractive_ty_size (T:=T1) ty1 ty2).
-      by f_equiv; apply type_contractive_ty_shr.
+  Global Instance product2_type_contractive {A B C} (T: _ A → _ B) (T': _ → _ C) :
+    TypeContractive T → TypeContractive T' → TypeContractive (λ ty, T ty * T' ty)%T.
+  Proof. move=> ??. split=>/=; first apply _.
+    - move=> *. f_equiv; by apply type_contractive_ty_size.
+    - move=> *. do 6 f_equiv; by apply type_contractive_ty_own.
+    - move=> ? ty ty' *. rewrite (type_contractive_ty_size (T:=T) ty ty').
+      f_equiv; by apply type_contractive_ty_shr.
   Qed.
 
-  Global Instance product2_ne {A B} : NonExpansive2 (@product2 A B).
-  Proof. solve_ne_type. Qed.
-
-End product.
-
-Notation "ty * ty'" := (product2 ty%T ty'%T) : lrust_type_scope.
-
-Section typing.
-  Context `{!typeG Σ}.
-
-  Global Instance product2_copy {A B} (ty1: _ A) (ty2: _ B) :
-    Copy ty1 → Copy ty2 → Copy (ty1 * ty2).
+  Global Instance cons_product2_type_ne {A B C} (T: _ A → _ B) (T': _ → _ C) :
+    TypeNonExpansive T → TypeNonExpansive T' → TypeNonExpansive (λ ty, T ty :* T' ty)%T.
   Proof.
-    move=> ??. split; first (intros; apply _).
-    intros vπd κ tid E F l q ? HF. iIntros "#LFT [H1 H2] Htl [Htok1 Htok2]".
-    iMod (@copy_shr_acc with "LFT H1 Htl Htok1")
-      as (q1 vl1) "(Htl & H↦1 & #H1 & Hclose1)"; first solve_ndisj.
-    { rewrite <-HF. apply shr_locsE_subseteq=>/=. lia. }
-    iMod (@copy_shr_acc with "LFT H2 Htl Htok2")
-      as (q2 vl2) "(Htl & H↦2 & #H2 & Hclose2)"; first solve_ndisj.
-    { move: HF. rewrite /= -plus_assoc shr_locsE_shift.
-      assert (shr_locsE l (ty_size ty1) ## shr_locsE (l +ₗ (ty_size ty1)) (ty_size ty2 + 1))
-             by exact: shr_locsE_disj.
-      set_solver. }
-    iDestruct (na_own_acc with "Htl") as "[$ Htlclose]".
-    { generalize (shr_locsE_shift l ty1.(ty_size) ty2.(ty_size))=>/=. set_solver+. }
-    destruct (Qp_lower_bound q1 q2) as (qq & q'1 & q'2 & -> & ->).
-    iExists qq, (vl1 ++ vl2). rewrite heap_mapsto_vec_app.
-    iDestruct (ty_size_eq with "H1") as ">->".
-    iDestruct "H↦1" as "[$ H↦1f]". iDestruct "H↦2" as "[$ H↦2f]".
-    iSplitR; [by simpl; eauto 10|]. iIntros "!> Htl [H↦1 H↦2]".
-    iDestruct ("Htlclose" with "Htl") as "Htl".
-    iMod ("Hclose2" with "Htl [H2 H↦2f H↦2]") as "[Htl $]"; [by iFrame|].
-    iApply ("Hclose1" with "Htl [H1 H↦1f H↦1]"). by iFrame.
+    have ->: (λ ty, T ty :* T' ty)%T =
+      mod_ty pair_to_cons_pair ∘ (λ ty, T ty * T' ty)%T by done.
+    move=> ??. apply type_ne_ne_compose; apply _.
+  Qed.
+  Global Instance cons_product2_type_contractive {A B C} (T: _ A → _ B) (T': _ → _ C) :
+    TypeContractive T → TypeContractive T' → TypeContractive (λ ty, T ty :* T' ty)%T.
+  Proof.
+    have ->: (λ ty, T ty :* T' ty)%T =
+      mod_ty pair_to_cons_pair ∘ (λ ty, T ty * T' ty)%T by done.
+    move=> ??. apply type_contractive_compose_left; apply _.
   Qed.
 
-  Global Instance product2_send {A B} (ty1: _ A) (ty2: _ B) :
-    Send ty1 → Send ty2 → Send (ty1 * ty2).
+  Global Instance product_type_ne {A Bs} (T: _ A → _ Bs) :
+    TypeListNonExpansive T → TypeNonExpansive (Π ∘ T).
   Proof.
-    move=> *?*. iDestruct 1 as (vl1 vl2 ->) "[Hown1 Hown2]".
-    iExists _, _. iSplit; first done. iSplitL "Hown1"; by iApply @send_change_tid.
+    move=> [Tl [Eq All]].
+    have ->: Π ∘ T = λ ty, Π ((λ _ (T': _ → _), T' ty) +<$>+ Tl).
+    { extensionality ty. by rewrite /= Eq. } clear Eq T.
+    dependent induction All=>/=; by [apply _|apply cons_product2_type_ne].
+  Qed.
+  Global Instance product_type_ne_cont {A Bs} (T: _ A → _ Bs) :
+    TypeListContractive T → TypeContractive (Π ∘ T).
+  Proof.
+    move=> [Tl [Eq All]].
+    have ->: Π ∘ T = λ ty, Π ((λ _ (T': _ → _), T' ty) +<$>+ Tl).
+    { extensionality ty. by rewrite /= Eq. } clear Eq T.
+    dependent induction All=>/=; by [apply _|apply cons_product2_type_contractive].
   Qed.
 
-  Global Instance product2_sync {A B} (ty1: _ A) (ty2: _ B) :
-    Sync ty1 → Sync ty2 → Sync (ty1 * ty2).
+  Global Instance product2_copy {A B} (ty: _ A) (ty': _ B) :
+    Copy ty → Copy ty' → Copy (ty * ty').
   Proof.
-    move=> *?*. iIntros "* [#Hshr1 #Hshr2]". iSplit; by iApply @sync_change_tid.
+    move=> ??. split; [by apply _|]=>/= > ? HF. iIntros "#LFT [Shr Shr'] Na [Tok Tok']".
+    iMod (copy_shr_acc with "LFT Shr Na Tok") as (q wl) "[Na[Mt[#Own Close]]]";
+    first done. { rewrite <-HF. apply shr_locsE_subseteq=>/=. lia. }
+    iMod (copy_shr_acc with "LFT Shr' Na Tok'") as (q' wl') "[Na[Mt'[#Own' Close']]]";
+    first done. { apply subseteq_difference_r. { symmetry. apply shr_locsE_disj. }
+      move: HF. rewrite -plus_assoc shr_locsE_shift. set_solver. }
+    iDestruct (na_own_acc with "Na") as "[$ PreNa]".
+    { rewrite shr_locsE_shift. set_solver. }
+    case (Qp_lower_bound q q')=> [qq[?[?[->->]]]].
+    iExists qq, (wl ++ wl'). rewrite heap_mapsto_vec_app.
+    iDestruct (ty_size_eq with "Own") as ">->".
+    iDestruct "Mt" as "[$ Mtr]". iDestruct "Mt'" as "[$ Mtr']".
+    iSplitR. { iIntros "!>!>". iExists wl, wl'. iSplit; by [|iSplit]. }
+    iIntros "!> Na [Mt Mt']". iDestruct ("PreNa" with "Na") as "Na".
+    iMod ("Close'" with "Na [$Mt' $Mtr']") as "[Na $]".
+    iApply ("Close" with "Na [$Mt $Mtr]").
   Qed.
+
+  Global Instance product2_send {A B} (ty: _ A) (ty': _ B) :
+    Send ty → Send ty' → Send (ty * ty').
+  Proof.
+    move=> *?*. iDestruct 1 as (wl wl' ->) "[Own Own']".
+    iExists wl, wl'. iSplit; [done|]. iSplitL "Own"; by iApply @send_change_tid.
+  Qed.
+  Global Instance product2_sync {A B} (ty: _ A) (ty': _ B) :
+    Sync ty → Sync ty' → Sync (ty * ty').
+  Proof.
+    move=> *?*. iIntros "[#? #?]". iSplit; by iApply @sync_change_tid.
+  Qed.
+
+  Global Instance product_copy {As} (tyl: _ As) : ListCopy tyl → Copy (Π tyl).
+  Proof. elim; apply _. Qed.
+  Global Instance product_send {As} (tyl: _ As) : ListSend tyl → Send (Π tyl).
+  Proof. elim; apply _. Qed.
+  Global Instance product_sync {As} (tyl: _ As) : ListSync tyl → Sync (Π tyl).
+  Proof. elim; apply _. Qed.
 
   Lemma product2_subtype {A B A' B'} E L (f: A → A') (g: B → B') ty1 ty2 ty1' ty2' :
     subtype E L f ty1 ty1' → subtype E L g ty2 ty2' →
     subtype E L (pair_map f g) (ty1 * ty2) (ty1' * ty2').
   Proof.
-    move=> H1 H2. iIntros (qL) "HL".
-    iDestruct (H1 with "HL") as "#H1". iDestruct (H2 with "HL") as "#H2".
-    iIntros "!> #HE".
-    iDestruct ("H1" with "HE") as "(% & #Hout1 & #Ho1 & #Hs1)". iClear (H1) "H1".
-    iDestruct ("H2" with "HE") as "(% & #Hout2 & #Ho2 & #Hs2)". iClear (H2) "H2".
-    iSplit; first by (iPureIntro; simpl; f_equal). iSplit; [|iSplit; iModIntro].
-    - rewrite !lft_intersect_list_app. by iApply lft_intersect_mono.
-    - iIntros (????) "H /=". iDestruct "H" as (vl1 vl2) "(-> & Hown1 & Hown2)".
-      iExists _, _. iSplit. done. iSplitL "Hown1".
-      + by iApply "Ho1".
-      + by iApply "Ho2".
-    - iIntros (?????) "/= #[Hshr1 Hshr2]". iSplit.
-      + by iApply "Hs1".
-      + rewrite -(_ : ty_size ty1 = ty_size ty1') //. by iApply "Hs2".
+    move=> Sub Sub'. iIntros (?) "L". iDestruct (Sub with "L") as "#Sub".
+    iDestruct (Sub' with "L") as "#Sub'". iIntros "!> #E".
+    iDestruct ("Sub" with "E") as (Eq) "[#InLft[#InOwn #InShr]]".
+    iDestruct ("Sub'" with "E") as (?) "[#InLft'[#InOwn' #InShr']]".
+    iSplit=>/=. { iPureIntro. by f_equal. } iSplit.
+    { rewrite !lft_intersect_list_app. by iApply lft_intersect_mono. }
+    iSplit; iModIntro.
+    - iIntros "*". iDestruct 1 as (wl wl' ->) "[Own Own']". iExists wl, wl'.
+      iSplit; [done|]. iSplitL "Own"; by [iApply "InOwn"|iApply "InOwn'"].
+    - iIntros "* #[??]". rewrite Eq. iSplit; by [iApply "InShr"|iApply "InShr'"].
   Qed.
 
   Lemma product2_eqtype {A B A' B'} E L (f: A → A') f' (g: B → B') g' ty1 ty2 ty1' ty2' :
     eqtype E L f f' ty1 ty1' → eqtype E L g g' ty2 ty2' →
     eqtype E L (pair_map f g) (pair_map f' g') (ty1 * ty2) (ty1' * ty2').
-  Proof. move=> [??] [??]. split; by apply product2_subtype. Qed.
+  Proof. move=> [??][??]. split; by apply product2_subtype. Qed.
 
-  (*
-  Definition product := foldr product2 unit0.
-  Definition unit := product [].
-
-  Lemma outlives_product ty1 ty2 ϝ :
-    ty_outlives_E (product [ty1; ty2]) ϝ = ty_outlives_E ty1 ϝ ++ ty_outlives_E ty2 ϝ.
-  Proof. rewrite /product /ty_outlives_E /= fmap_app right_id //. Qed.
-
-  Global Instance product_type_ne Tl:
-    TypeListNonExpansive Tl → TypeNonExpansive (product ∘ Tl).
+  Lemma cons_product2_subtype {A B A' B'} E L (f: A → A') (g: B → B') ty1 ty2 ty1' ty2' :
+    subtype E L f ty1 ty1' → subtype E L g ty2 ty2' →
+    subtype E L (cons_pair_map f g) (ty1 :* ty2) (ty1' :* ty2').
   Proof.
-    intros (Tl' & HTlTl' & HTl').
-    eapply type_ne_ext; last first.
-    { intros ty. by rewrite /= HTlTl'. }
-    clear Tl HTlTl'. induction HTl' as [|T Tl'  HT HTl' ]=>/=; apply _.
+    move=> ??. rewrite cons_pair_map_via_pair_map. apply mod_ty_subtype.
+    { apply pair_via_cons_pair. } by apply product2_subtype.
   Qed.
-  Global Instance product_type_ne_cont Tl:
-    TypeListContractive Tl → TypeContractive (product ∘ Tl).
+
+  Lemma product_subtype {As Bs} E L (tyl: _ As) (tyl': _ Bs) fl :
+    subtypel E L tyl tyl' fl → subtype E L (xprod_map fl) (Π tyl) (Π tyl').
   Proof.
-    intros (Tl' & HTlTl' & HTl').
-    eapply type_contractive_ext; last first.
-    { intros ty. by rewrite /= HTlTl'. }
-    clear Tl HTlTl'. induction HTl' as [|T Tl'  HT HTl' ]=>/=; apply _.
+    move=> Subs. dependent induction Subs; [by apply subtype_refl|].
+    by apply cons_product2_subtype.
   Qed.
-  Global Instance product_ne : NonExpansive product.
-  Proof. intros ??. induction 1=>//=. by f_equiv. Qed.
-  Global Instance product_mono E L:
-    Proper (Forall2 (subtype E L) ==> subtype E L) product.
-  Proof. intros ??. induction 1=>//=. by f_equiv. Qed.
-  Lemma product_mono' E L tyl1 tyl2 :
-    Forall2 (subtype E L) tyl1 tyl2 → subtype E L (product tyl1) (product tyl2).
-  Proof. apply product_mono. Qed.
-  Global Instance product_proper E L:
-    Proper (Forall2 (eqtype E L) ==> eqtype E L) product.
-  Proof. intros ??. induction 1=>//=. by f_equiv. Qed.
-  Lemma product_proper' E L tyl1 tyl2 :
-    Forall2 (eqtype E L) tyl1 tyl2 → eqtype E L (product tyl1) (product tyl2).
-  Proof. apply product_proper. Qed.
-  Global Instance product_copy tys : ListCopy tys → Copy (product tys).
-  Proof. induction 1; apply _. Qed.
-  Global Instance product_send tys : ListSend tys → Send (product tys).
-  Proof. induction 1; apply _. Qed.
-  Global Instance product_sync tys : ListSync tys → Sync (product tys).
-  Proof. induction 1; apply _. Qed.
 
-  Definition product_cons ty tyl :
-    product (ty :: tyl) = product2 ty (product tyl) := eq_refl _.
-  Definition product_nil :
-    product [] = unit0 := eq_refl _.
+  Lemma product_eqtype {As Bs} E L (tyl: _ As) (tyl': _ Bs) fl gl :
+    eqtypel E L tyl tyl' fl gl →
+    eqtype E L (xprod_map fl) (xprod_map gl) (Π tyl) (Π tyl').
+  Proof.
+    move=> /HForallZip_zip [? /HForallZip_flip ?]. by split; apply product_subtype.
+  Qed.
 
-Notation Π := product.
+  Lemma outlives_product2 {A B} (ty: _ A) (ty': _ B) ϝ :
+    ty_outlives_E (ty * ty') ϝ = ty_outlives_E ty ϝ ++ ty_outlives_E ty' ϝ.
+  Proof. by rewrite /ty_outlives_E /= fmap_app. Qed.
 
+(*
   Global Instance prod2_assoc E L : Assoc (eqtype E L) product2.
   Proof.
     intros ???. apply eqtype_unfold. iIntros (?) "_ !> _".
